minor cleanup

src/Std/Data/DTreeMap/Internal/Zipper.lean
@@ -254,8 +254,7 @@ public instance Zipper.instFinite : Finite (Zipper α β) Id :=
   .of_finitenessRelation Zipper.instFinitenessRelation
 
 @[always_inline]
-public def Zipper.iter (t : Zipper α β) : Iter (α := Zipper α β) ((a : α) × β a) :=
-  ⟨t⟩
+public def Zipper.iter (t : Zipper α β) : Iter (α := Zipper α β) ((a : α) × β a) := ⟨t⟩
 
 public def Zipper.iter_of_tree (t : Impl α β) : Iter (α := Zipper α β) ((a : α) × β a) :=
   Zipper.iter <| Zipper.done.prependMap t
@@ -313,7 +312,7 @@ public theorem Zipper.val_step_Zipper_eq_match {α β}
         Iter.mk.injEq, Sigma.mk.injEq]
       simp_all
 
-public theorem Zipper.toList_iter {α β} {z : Zipper α β}: z.iter.toList = z.toList := by
+@[simp] public theorem Zipper.toList_iter {α β} {z : Zipper α β}: z.iter.toList = z.toList := by
   rw [Iter.toList_eq_match_step]
   generalize hit : (z.iter.step.val) = step
   rw [val_step_Zipper_eq_match] at hit
@@ -396,58 +395,6 @@ public theorem Zipper.val_step_map_Zipper_eq_match {α β γ} {f : (a : α) × �
   rcases x with ⟨val, prop⟩
   simp [heq] at this
   split at this <;> (rename_i heq2 ; simp [heq2, this])
-
--- public theorem Zipper.toList_map_Zipper {α β γ} {f : (a : α) × β a → γ}
---     {z : Zipper α β}:
---     ((⟨z⟩ : Iter (Sigma β)).map f).toList =
---       (z.toList).map f := by
---   rw [Iter.toList_eq_match_step]
---   generalize hit : ((⟨z⟩ : Iter (Sigma β)).map f).step.val = step
---   rw [val_step_map_Zipper_eq_match] at hit
---   simp only at hit
---   split at hit
---   case h_1 x heq =>
---     simp only [← hit, List.nil_eq]
---     cases z
---     . simp only [Zipper.toList, List.map_nil]
---     . simp only [Zipper.iter, Iter.mk.injEq, reduceCtorEq] at heq
---   case h_2 =>
---     rename_i x k v t z' heq
---     simp only [← hit]
---     have := @Zipper.toList_iter _ _ (prependMap t z')
---     simp only [Zipper.iter] at this
-
---     rw [← this]
---     . generalize heq2 : Zipper.cons k v t z' = y
---       rw [heq2] at heq
---       simp only [Zipper.iter, Iter.mk.injEq] at heq
---       rw [heq]
---       rw [← heq2]
---       conv =>
---         rhs
---         rw [toList_Zipper]
---       simp only [Iter.toList_map, Zipper.toList, List.cons_append, List.map_cons]
---       simp only [← Zipper.prependMap_toList_eq_concat_toList, List.cons.injEq, true_and]
---       rw [←toList_map_Zipper]
---       simp
---   termination_by z.size
---   decreasing_by
---     simp_all
---     rename_i k v t z' _ heq
---     simp only [Zipper.iter, Iter.mk.injEq] at heq
---     rw [heq]
---     simp only [Zipper.size]
---     induction t
---     case leaf =>
---       simp only [Zipper.prependMap, Impl.treeSize, Nat.add_zero, Nat.lt_add_left_iff_pos,
---         Nat.lt_add_one]
---     case inner =>
---       simp only [Zipper.prependMap_size, Impl.treeSize, Nat.add_lt_add_iff_right, Nat.lt_add_left_iff_pos,
---         Nat.lt_add_one]
-
-public theorem Zipper.iter_of_tree_internal_state_eq {m : Impl α β} :
-    (Zipper.iter_of_tree m).internalState = Zipper.prependMap m .done := by
-  simp [Zipper.iter_of_tree, Zipper.iter]
 
 end Zipper
 
